pulse/lib/pulse/lib/Pulse.Lib.ArrayPtr.fst
@@ -65,7 +65,7 @@ fn from_array (#t: Type) (a: A.array t) (#p: perm) (#v: Ghost.erased (Seq.seq t)
     A.pts_to_range_intro a p v;
     rewrite (A.pts_to_range a 0 (A.length a) #p v)
         as (A.pts_to_range res.base (SZ.v res.offset) (SZ.v res.offset + Seq.length v) #p v);
-    fold_pts_to res #p v;
+    fold pts_to res #p v;
     res
 }
 
@@ -75,7 +75,7 @@ fn to_array (#t: Type) (s: ptr t) (a: array t) (#p: perm) (#v: Seq.seq t)
     ensures A.pts_to a #p v
 {
     unfold is_from_array s (Seq.length v) a;
-    unfold_pts_to s #p v;
+    unfold pts_to s #p v;
     A.pts_to_range_prop s.base;
     rewrite (A.pts_to_range s.base (SZ.v s.offset) (SZ.v s.offset + Seq.length v) #p v)
         as (A.pts_to_range a 0 (A.length a) #p v);
@@ -97,12 +97,14 @@ fn op_Array_Access
               SZ.v i < Seq.length s /\
               res == Seq.index s (SZ.v i))
 {
-    unfold_pts_to a #p s;
+    unfold pts_to a #p s;
     A.pts_to_range_prop a.base;
     let res = A.pts_to_range_index a.base (SZ.add a.offset i);
-    fold_pts_to a #p s;
+    fold pts_to a #p s;
     res
 }
+
+#set-options "--print_implicits"
 
 fn op_Array_Assignment
         (#t: Type)
@@ -118,10 +120,15 @@ fn op_Array_Assignment
               s' == Seq.upd s (SZ.v i) v
             )
 {
-    unfold_pts_to a s;
+    unfold pts_to a s;
     A.pts_to_range_prop a.base;
     let res = A.pts_to_range_upd a.base (SZ.add a.offset i) v;
-    fold_pts_to a (Seq.upd s (SZ.v i) v);
+    rewrite
+      A.pts_to_range a.base (SZ.v a.offset) (SZ.v a.offset + Seq.length s) (Seq.upd s (SZ.v i) v)
+    as
+      A.pts_to_range a.base (SZ.v a.offset) (SZ.v a.offset + Seq.length (Seq.upd s (SZ.v i) v)) (Seq.upd s (SZ.v i) v);
+    fold pts_to a (Seq.upd s (SZ.v i) v);
+    ();
 }
 
 ghost
@@ -133,10 +140,10 @@ fn share
   requires pts_to arr #p s
   ensures pts_to arr #(p /. 2.0R) s ** pts_to arr #(p /. 2.0R) s
 {
-    unfold_pts_to arr #p s;
+    unfold pts_to arr #p s;
     A.pts_to_range_share arr.base;
-    fold_pts_to arr #(p /. 2.0R) s;
-    fold_pts_to arr #(p /. 2.0R) s;    
+    fold pts_to arr #(p /. 2.0R) s;
+    fold pts_to arr #(p /. 2.0R) s;
 }
 
 ghost
@@ -148,10 +155,11 @@ fn gather
   requires pts_to arr #p0 s0 ** pts_to arr #p1 s1 ** pure (Seq.length s0 == Seq.length s1)
   ensures pts_to arr #(p0 +. p1) s0 ** pure (s0 == s1)
 {
-    unfold_pts_to arr #p0 s0;
-    unfold_pts_to arr #p1 s1;
-    A.pts_to_range_gather arr.base;
-    fold_pts_to arr #(p0 +. p1) s0
+    unfold pts_to arr #p0 s0;
+    unfold pts_to arr #p1 s1;
+    rewrite each Seq.length s1 as Seq.length s0;
+    A.pts_to_range_gather arr.base #_ #_ #s0 #s1 #p0 #p1;
+    fold pts_to arr #(p0 +. p1) s0
 }
 
 fn split (#t: Type) (s: ptr t) (#p: perm) (i: SZ.t)
@@ -174,7 +182,7 @@ fn split (#t: Type) (s: ptr t) (#p: perm) (i: SZ.t)
     rewrite
         (A.pts_to_range s.base (SZ.v s.offset) (SZ.v s'.offset) #p s1)
         as (A.pts_to_range s.base (SZ.v s.offset) (SZ.v s.offset + SZ.v i) #p s1);
-    fold_pts_to s #p s1;  
+    fold pts_to s #p s1;
     with s2. assert A.pts_to_range s.base (SZ.v s'.offset) (SZ.v s.offset + Seq.length v) #p s2;
     rewrite
         (A.pts_to_range s.base (SZ.v s'.offset) (SZ.v s.offset + Seq.length v) #p s2)
