pulse/lib/pulse/lib/Pulse.Lib.Task.fst
@@ -49,7 +49,7 @@ let v (s : task_state) : int =
   | Running -> 1
   | Done -> 2
   | Claimed -> 3
-  
+
 let p_st : preorder task_state = fun x y -> b2t (v x <= v y)
 
 let anchor_rel : FRAP.anchor_rel p_st =
@@ -69,7 +69,7 @@ let anchor_rel_refl (x:task_state) :
 let state_res
   (pre : slprop)
   (post : slprop)
-  (g_state : AR.ref task_state p_st anchor_rel)
+  ([@@@mkey] g_state : AR.ref task_state p_st anchor_rel)
   (st : task_state)
 =
   match st with
@@ -101,7 +101,7 @@ type task_t : Type0 = {
 let state_pred
   (pre : slprop_ref)
   (post : slprop_ref)
-  (h : handle)
+  ([@@@mkey] h : handle)
 : slprop =
   exists* (v_state : task_state).
     pts_to
@@ -140,6 +140,7 @@ ghost fn task_thunk_typing_dup t
 instance task_thunk_typing_duplicable t : duplicable (task_thunk_typing t) =
   { dup_f = fun _ -> task_thunk_typing_dup t }
 
+[@@no_mkeys] (* usually there's only a single instance *)
 let rec all_state_pred
   ( v_runnable : list task_t)
 : slprop
@@ -395,9 +396,10 @@ fn rec extract_state_pred
         {
           add_one_state_pred t' ts';
         };
-        intro_trade (state_pred t.pre t.post t.h) (all_state_pred ts)
-                    (pure (ts == t'::ts') ** task_thunk_typing t' ** all_state_pred ts') aux;
-
+        intro_trade
+          (state_pred t.pre t.post t.h) (all_state_pred ts)
+          (pure (ts == t::ts') ** task_thunk_typing t ** all_state_pred ts')
+          aux;
         ()
       }
     }
@@ -511,8 +513,10 @@ fn spawn (p:pool)
     post = post_ref;
     thunk = Dyn.mkdyn f;
   };
-  dup (slprop_ref_pts_to post_ref post) ();
-  dup (slprop_ref_pts_to pre_ref pre) ();
+  rewrite each pre_ref as task.pre;
+  rewrite each post_ref as task.post;
+  dup (slprop_ref_pts_to task.pre pre) ();
+  dup (slprop_ref_pts_to task.post post) ();
   fold task_thunk_typing_core task pre post;
   fold task_thunk_typing task;
   
@@ -611,7 +615,7 @@ fn try_await
   AR.drop_anchor p.g_runnable;
   recall_task_spotted p t #v_runnable;
   AR.lift_anchor p.g_runnable _;
-  
+
   extract_state_pred p t #v_runnable;
 
   let v_state = elim_state_pred t.pre t.post t.h;
@@ -619,7 +623,7 @@ fn try_await
   rewrite (pts_to t.h.state #(if Running? v_state then 0.5R else 1.0R) (unclaimed (reveal v_state)))
        as (pts_to h.state #(if Running? v_state then 0.5R else 1.0R) (unclaimed (reveal v_state)));
   let task_st = !h.state;
-  
+
   match task_st {
     Ready -> {
       (* NOOP *)
@@ -650,25 +654,16 @@ fn try_await
     Done -> {
       (* First prove that ghost state cannot be Claimed,
       due to the anchor *)
-      rewrite (AR.pts_to t.h.g_state v_state)
-           as (AR.pts_to h.g_state v_state);
-      assert (AR.pts_to h.g_state v_state);
-      assert (AR.anchored h.g_state Ready);
-      AR.recall_anchor h.g_state Ready;
+      rewrite each h as t.h;
+      AR.recall_anchor t.h.g_state Ready;
       assert (pure (v_state =!= Claimed));
       assert (pure (v_state == Done));
-      rewrite (AR.pts_to h.g_state v_state)
-           as (AR.pts_to t.h.g_state v_state);
 
       (* Now claim it *)
       claim_done_task #p #(up t.pre) #(up t.post) t.h;
 
       gtrade_elim (up t.post ** later_credit 1) post;
-      rewrite (post)
-           as (if true then post else joinable p post h);
-           
-      rewrite (pts_to h.state Done)
-           as (pts_to t.h.state (unclaimed Claimed));
+
       intro_state_pred t.pre t.post t.h Claimed;
       elim_trade _ _; // undo extract_state_pred
       fold (lock_inv p.runnable p.g_runnable);
@@ -692,6 +687,7 @@ let handle_done (h:handle) : slprop =
 let task_done (t : task_t)  : slprop =
   handle_done t.h
 
+[@@no_mkeys] (* usually there's only a single instance *)
 let rec all_tasks_done (ts : list task_t) =
   match ts with
   | [] -> emp
@@ -818,6 +814,7 @@ fn disown_aux
 
   match st {
     Done -> {
+      rewrite each h as t.h;
       rewrite (state_res (up t.pre) (up t.post) t.h.g_state Done)
            as up t.post;
 
@@ -843,6 +840,7 @@ fn disown_aux
     }
     Claimed -> {
       assert (AR.anchored h.g_state Ready);
+      rewrite each h as t.h;
       AR.recall_anchor t.h.g_state Ready;
       unreachable();
     }
@@ -904,9 +902,14 @@ fn await (#p:pool)
         (if v_done then post else joinable p post h) **
         pure (b == not v_done)
   {
+    with v_done. assert (pts_to done v_done);
+    rewrite each v_done as false;
     let b = try_await #p #post h #f;
     done := b;
   };
+  with v_done. assert (pts_to done v_done);
+  rewrite each v_done as true;
+  ()
 }
 
 ghost
@@ -1022,15 +1025,14 @@ fn weaken_vopt (#a:Type0) (o : option a)
 {
   match o {
     None -> {
-      unfold (vopt None p1);
-      fold (vopt None p2);
+      rewrite vopt None p1 as vopt o p2;
       drop_ extra;
       ()
     }
     Some v -> {
-      rewrite (vopt o p1) as p1 v;
+      unfold vopt (Some v) p1;
       f v;
-      fold (vopt o p2);
+      rewrite p2 v as vopt o p2;
     }
   }
 }
@@ -1109,7 +1111,9 @@ fn rec grab_work' (p:pool)
              up t.pre ** pts_to t.h.state #0.5R Running ** task_spotted p t ** task_thunk_typing t)
 {
   unfold (lock_inv p.runnable p.g_runnable);
+  with v_runnable0. assert (pts_to p.runnable v_runnable0);
   let v_runnable = !p.runnable;
+  rewrite each v_runnable0 as v_runnable;
   let topt = grab_work'' p v_runnable;
 
   AR.take_snapshot_full p.g_runnable;
@@ -1212,11 +1216,9 @@ fn do_work_once (#f:perm) (p : pool)
   let topt = grab_work p;
   match topt {
     None -> {
-      rewrite (if Some? topt then up (Some?.v topt).pre else emp)
-           as emp;
+      unfold (vopt #task_t);
     }
     Some t -> {
-      rewrite each topt as Some t;
       get_vopt #task_t #t ();
       perf_work t;
       put_back_result p t
@@ -1251,12 +1253,18 @@ fn await_help
         (if v_done then post else joinable p post h) **
         pure (b == not v_done)
   {
+    with v_done. assert (pts_to done v_done);
+    rewrite each v_done as false;
     let b = try_await #p #post h #f;
     done := b;
     if (not b) {
       do_work_once #f p;
     }
   };
+  with v_done.
+    assert (pts_to done v_done);
+    rewrite each v_done as true;
+  ();
 }
 
 let ite (b:bool) (p q : slprop) : slprop =
@@ -1282,7 +1290,7 @@ fn rec check_if_all_done
         Done -> {
           let bb = check_if_all_done ts';
           if bb {
-            rewrite (ite bb (all_tasks_done ts') emp) as (all_tasks_done ts');
+            rewrite ite true (all_tasks_done ts') emp as (all_tasks_done ts');
             with g_st. assert (AR.pts_to t.h.g_state g_st);
             assert (pure (g_st == Done \/ g_st == Claimed));
             AR.take_snapshot t.h.g_state;
@@ -1293,7 +1301,7 @@ fn rec check_if_all_done
             add_one_state_pred t ts';
             true;
           } else {
-            drop_ (ite bb (all_tasks_done ts') emp);
+            drop_ (ite false (all_tasks_done ts') emp);
             fold (state_pred t.pre t.post t.h);
             add_one_state_pred t ts';
             rewrite emp as ite false (all_tasks_done ts) emp;
@@ -1411,9 +1419,8 @@ fn rec teardown_pool
 
   let runnable = !p.runnable;
   let b = check_if_all_done runnable;
+  unfold ite;
   if b {
-    rewrite ite b (all_tasks_done runnable) emp
-         as all_tasks_done runnable;
     AR.drop_anchor p.g_runnable;
     AR.share p.g_runnable;
     fold (pool_done p);
@@ -1427,8 +1434,6 @@ fn rec teardown_pool
     drop_ (lock_alive _ #0.5R _);
     drop_ (lock_acquired p.lk);
   } else {
-    rewrite ite b (all_tasks_done runnable) emp
-         as emp;
     (* Spin *)
     fold (lock_inv p.runnable p.g_runnable);
     release p.lk;
